remove option from Memory

src/Memory.v
@@ -1,187 +1,68 @@
-(* import List before bbv.Word, otherwise Word.combine gets shadowed and huge type class
-   inference failure messages will appear *)
-Require Import Coq.Lists.List.
-Require Import Coq.omega.Omega.
 Require Import bbv.Word.
-Require Import Coq.ZArith.BinInt.
-Require Import riscv.util.Decidable.
-Require Import riscv.Utility.
-Require Import riscv.util.Monads.
 
-(* TODO remove option here, making it very simple,
-   and only use option based memory in compiler *)
 Class Memory(m: Set)(a: Set) := mkMemory {
-  loadByte : m -> a -> option (word 8);
-  loadHalf : m -> a -> option (word 16);
-  loadWord : m -> a -> option (word 32);
-  loadDouble : m -> a -> option (word 64);
-  storeByte : m -> a -> word 8 -> option m;
-  storeHalf : m -> a -> word 16 -> option m;
-  storeWord : m -> a -> word 32 -> option m;
-  storeDouble : m -> a -> word 64 -> option m;
+  loadByte   : m -> a -> word  8;
+  loadHalf   : m -> a -> word 16;
+  loadWord   : m -> a -> word 32;
+  loadDouble : m -> a -> word 64;
+  storeByte  : m -> a -> word  8 -> m;
+  storeHalf  : m -> a -> word 16 -> m;
+  storeWord  : m -> a -> word 32 -> m;
+  storeDouble: m -> a -> word 64 -> m;
 }.
 
-(* memory addresses are represented using Z because word does not restrict them enough,
-   there are always invalid memory addresses, which are represented by returning None,
-   so we prefer Z, also because that's more "high-level computation" related, where we
-   use Z, rather than "store state" related, where we use word *)
-
-Local Open Scope Z_scope.
-
-Section Memory.
-
-  Variable w: nat. (* bit width of memory words *)
-
-  Definition mem := Z -> option (word w).
-
-  Definition read_mem(x: Z)(m: mem): option (word w) := m x.
-
-  Definition write_mem(x: Z)(v: word w)(m: mem): option mem :=
-    match m x with
-    | Some old_value => Some (fun y => if dec (x = y) then Some v else m y)
-    | None => None
-    end.
-
-  Definition no_mem: mem := fun x => None.
-
-  Definition const_mem(size: Z)(default: word w): mem :=
-    fun x => if dec (x < size) then Some default else None.
-
-  Definition zero_mem(size: Z): mem := const_mem size $0.
-
-  Definition counter_mem(size: Z): mem :=
-    fun x => if dec (x < size) then Some (ZToWord w x) else None.
-
-End Memory.
-
-Arguments read_mem {_} _.
-Arguments write_mem {_} _ _.
-
-Definition read_byte(m: mem 8)(a: Z): option (word 8) := read_mem a m.
-Definition read_half(m: mem 8)(a: Z): option (word 16) :=
-  v0 <- read_byte m a; v1 <- read_byte m (a + 1); Return (combine v0 v1).
-Definition read_word(m: mem 8)(a: Z): option (word 32) :=
-  v0 <- read_half m a; v1 <- read_half m (a + 2); Return (combine v0 v1).
-Definition read_double(m: mem 8)(a: Z): option (word 64) :=
-  v0 <- read_word m a; v1 <- read_word m (a + 4); Return (combine v0 v1).
-
-Definition lobits(sz: nat)(w: word (sz + sz)): word sz := split1 sz sz w.
-Definition hibits(sz: nat)(w: word (sz + sz)): word sz := split2 sz sz w.
-
-Definition write_byte(m: mem 8)(a: Z)(v: word 8): option (mem 8) := write_mem a v m.
-Definition write_half(m: mem 8)(a: Z)(v: word 16): option (mem 8) :=
-  m <- write_byte m a (lobits 8 v); write_byte m (a + 1) (hibits 8 v).
-Definition write_word(m: mem 8)(a: Z)(v: word 32): option (mem 8) :=
-  m <- write_half m a (lobits 16 v); write_half m (a + 2) (hibits 16 v).
-Definition write_double(m: mem 8)(a: Z)(v: word 64): option (mem 8) :=
-  m <- write_word m a (lobits 32 v); write_word m (a + 4) (hibits 32 v).
-
-
-Definition uwordToZ{sz: nat}(w: word sz): Z := Z.of_N (wordToN w).
-
-Definition wrapLoad{aw sz: nat}(f: mem 8 -> Z -> option (word sz))
-  (m: mem 8)(a: word aw): option (word sz) := f m (uwordToZ a).
-
-Definition wrapStore{aw sz: nat}(f: mem 8 -> Z -> word sz -> option (mem 8))
-  (m: mem 8)(a: word aw)(v: word sz): option (mem 8) := f m (uwordToZ a) v.
-
-Instance mem_is_Memory(aw: nat): Memory (mem 8) (word aw) := {|
-  loadByte   := wrapLoad read_byte;
-  loadHalf   := wrapLoad read_half;
-  loadWord   := wrapLoad read_word;
-  loadDouble := wrapLoad read_double;
-  storeByte   := wrapStore write_byte;
-  storeHalf   := wrapStore write_half;
-  storeWord   := wrapStore write_word;
-  storeDouble := wrapStore write_double;
-|}.
-
-
-Section store_retrieve.
+Section MemoryHelpers.
 
   Context {sz: nat}.
+  Context {Mem: Set}.
+  Context {MM: Memory Mem (word sz)}.
 
-  Fixpoint storeWords(l: list (word 32))(a: word sz)(m: mem 8): option (mem 8) :=
+  Fixpoint store_byte_list(l: list (word 8))(a: word sz)(m: Mem): Mem :=
     match l with
-    | nil => Some m
-    | cons w l' =>
-        match storeWord m a w with
-        | Some m' => storeWords l' (a ^+ $4) m'
-        | None => None
-        end
+    | nil => m
+    | cons w l' => let m' := storeByte m a w in store_byte_list l' (a ^+ $1) m'
     end.
 
-  Fixpoint mem_to_word_list(m: mem 8)(start: Z)(count: nat): list (option (word 32)) :=
+  Fixpoint load_byte_list(m: Mem)(start: word sz)(count: nat): list (word 8) :=
     match count with
-    | S c => read_word m start :: mem_to_word_list m (start + 4) c
+    | S c => loadByte m start :: load_byte_list m (start ^+ $1) c
     | O => nil
     end.
 
-  Lemma write_read_byte: forall m m' a v ,
-    write_byte m a v = Some m' ->
-    read_byte m' a = Some v.
-  Proof.
-    intros. unfold write_byte, read_byte, read_mem, write_mem in *.
-    destruct (m a) eqn: E; [|discriminate].
-    inversion H. clear H. subst.
-    match goal with
-    | |- context [@dec ?P ?d] =>
-      let x := constr:(@dec P d) in destruct x; [reflexivity|contradiction]
+  Fixpoint store_half_list(l: list (word 16))(a: word sz)(m: Mem): Mem :=
+    match l with
+    | nil => m
+    | cons w l' => let m' := storeHalf m a w in store_half_list l' (a ^+ $2) m'
     end.
-  Qed.
 
-  Lemma write_read_byte_diff: forall a1 a2 m m' v o,
-    a2 <> a1 ->
-    read_byte m a1 = o ->
-    write_byte m a2 v = Some m' ->
-    read_byte m' a1 = o.
-  Proof.
-    intros. unfold read_byte, write_byte, read_mem, write_mem in *.
-    destruct (m a2) eqn: E; [|discriminate].
-    inversion H1.
-    match goal with
-    | |- context [@dec ?P ?d] =>
-      let x := constr:(@dec P d) in destruct x; [contradiction|assumption]
+  Fixpoint load_half_list(m: Mem)(start: word sz)(count: nat): list (word 16) :=
+    match count with
+    | S c => loadHalf m start :: load_half_list m (start ^+ $2) c
+    | O => nil
     end.
-  Qed.
 
-  Lemma write_read_half: forall m m' a v ,
-    write_half m a v = Some m' ->
-    read_half m' a = Some v.
-  Proof.
-    intros. unfold write_half, read_half in *. simpl in *.
-    match goal with
-    | H: match ?x with _ => _ end = Some _ |- _ => destruct x eqn: E; [|discriminate]
+  Fixpoint store_word_list(l: list (word 32))(a: word sz)(m: Mem): Mem :=
+    match l with
+    | nil => m
+    | cons w l' => let m' := storeWord m a w in store_word_list l' (a ^+ $4) m'
     end.
-    pose proof H as H'.
-    apply write_read_byte in H'. rewrite H'.
-    pose proof E as E'.
-    apply write_read_byte in E'.
-    assert (a + 1 <> a) as Q by omega.
-    pose proof (write_read_byte_diff a _ m0 m' _ _ Q E' H) as P.
-    rewrite P.
-    f_equal.
-    unfold lobits, hibits.
-    apply combine_split.
-  Qed.
 
-  Lemma write_read_word: forall m m' a v ,
-    write_word m a v = Some m' ->
-    read_word m' a = Some v.
-  Admitted.
+  Fixpoint load_word_list(m: Mem)(start: word sz)(count: nat): list (word 32) :=
+    match count with
+    | S c => loadWord m start :: load_word_list m (start ^+ $4) c
+    | O => nil
+    end.
 
-  Lemma store_retrieve_word_list: forall l a m m',
-    storeWords l a m = Some m' ->
-    mem_to_word_list m' (uwordToZ a) (length l) = map Some l.
-  Proof.
-    induction l; intros; simpl in *; try reflexivity.
-    destruct (wrapStore write_word m a0 a) eqn: F; [|discriminate].
-    specialize IHl with (1 := H).
-    assert (uwordToZ (a0 ^+ $4) = uwordToZ a0 + 4) as E by admit.
-    rewrite E in IHl.
-    rewrite IHl.
-    f_equal.
-    unfold wrapStore in F.
-  Abort.
+  Fixpoint store_double_list(l: list (word 64))(a: word sz)(m: Mem): Mem :=
+    match l with
+    | nil => m
+    | cons w l' => let m' := storeDouble m a w in store_double_list l' (a ^+ $8) m'
+    end.
 
-End store_retrieve.
+  Fixpoint load_double_list(m: Mem)(start: word sz)(count: nat): list (word 64) :=
+    match count with
+    | S c => loadDouble m start :: load_double_list m (start ^+ $8) c
+    | O => nil
+    end.
+
+End MemoryHelpers.
