src/FunctionMemory.v
@@ -1,0 +1,85 @@
+(* import List before bbv.Word, otherwise Word.combine gets shadowed and huge type class
+   inference failure messages will appear *)
+Require Import Coq.Lists.List.
+Require Import Coq.omega.Omega.
+Require Import bbv.Word.
+Require Import Coq.ZArith.BinInt.
+Require Import riscv.util.Decidable.
+Require Import riscv.Utility.
+Require Import riscv.util.Monads.
+Require Import riscv.Memory.
+
+Local Open Scope Z_scope.
+
+Section Memory.
+
+  Context {w: nat}. (* bit width of memory addresses *)
+
+  Definition mem := word w -> word 8.
+
+  Definition read_byte(m: mem)(a: word w): word 8 := m a.
+  Definition read_half(m: mem)(a: word w): word 16 :=
+    let v0 := read_byte m a in let v1 := read_byte m (a ^+ $1) in combine v0 v1.
+  Definition read_word(m: mem)(a: word w): word 32 :=
+    let v0 := read_half m a in let v1 := read_half m (a ^+ $2) in combine v0 v1.
+  Definition read_double(m: mem)(a: word w): word 64 :=
+    let v0 := read_word m a in let v1 := read_word m (a ^+ $4) in combine v0 v1.
+
+  Definition lobits(sz: nat)(w: word (sz + sz)): word sz := split1 sz sz w.
+  Definition hibits(sz: nat)(w: word (sz + sz)): word sz := split2 sz sz w.
+
+  Definition write_byte(m: mem)(a: word w)(v: word 8): mem :=
+    fun a' => if weq a' a then v else m a'.
+  Definition write_half(m: mem)(a: word w)(v: word 16): mem :=
+    let m := write_byte m a (lobits 8 v) in write_byte m (a ^+ $1) (hibits 8 v).
+  Definition write_word(m: mem)(a: word w)(v: word 32): mem :=
+    let m := write_half m a (lobits 16 v) in write_half m (a ^+ $2) (hibits 16 v).
+  Definition write_double(m: mem)(a: word w)(v: word 64): mem :=
+    let m := write_word m a (lobits 32 v) in write_word m (a ^+ $4) (hibits 32 v).
+
+  Definition const_mem(default: word 8): mem := fun a => default.
+
+  Definition zero_mem: mem := const_mem $0.
+
+End Memory.
+
+Arguments mem : clear implicits.
+
+
+Instance mem_is_Memory(w: nat): Memory (mem w) (word w) := {|
+  loadByte    := read_byte;
+  loadHalf    := read_half;
+  loadWord    := read_word;
+  loadDouble  := read_double;
+  storeByte   := write_byte;
+  storeHalf   := write_half;
+  storeWord   := write_word;
+  storeDouble := write_double;
+|}.
+
+Lemma write_read_byte: forall sz m (a: word sz) v ,
+  read_byte (write_byte m a v) a = v.
+Proof.
+  intros. unfold write_byte, read_byte in *.
+  simpl.
+  rewrite (rewrite_weq eq_refl). reflexivity.
+Qed.
+
+Lemma write_read_byte_diff: forall sz (a1 a2: word sz) m v,
+  a2 <> a1 ->
+  read_byte (write_byte m a2 v) a1 = read_byte m a1.
+Proof.
+  intros. unfold read_byte, write_byte in *.
+  destruct (weq a1 a2); congruence.
+Qed.
+
+Lemma write_read_half: forall sz m (a: word (S sz)) v ,
+  read_half (write_half m a v) a = v.
+Proof.
+  intros. unfold write_half, read_half in *.
+  rewrite (write_read_byte _ (write_byte m a (lobits 8 v)) (a ^+ $1) (hibits 8 v)).
+  assert (a ^+ $1 <> a) as Q by apply wplus_one_neq.
+  rewrite (write_read_byte_diff _ a (a ^+ $1) _ (hibits 8 v) Q).
+  rewrite write_read_byte.
+  apply (combine_split 8 8).
+Qed.
