src/Memory_Option.v
@@ -1,0 +1,187 @@
+(* import List before bbv.Word, otherwise Word.combine gets shadowed and huge type class
+   inference failure messages will appear *)
+Require Import Coq.Lists.List.
+Require Import Coq.omega.Omega.
+Require Import bbv.Word.
+Require Import Coq.ZArith.BinInt.
+Require Import riscv.util.Decidable.
+Require Import riscv.Utility.
+Require Import riscv.util.Monads.
+
+(* TODO remove option here, making it very simple,
+   and only use option based memory in compiler *)
+Class Memory(m: Set)(a: Set) := mkMemory {
+  loadByte : m -> a -> option (word 8);
+  loadHalf : m -> a -> option (word 16);
+  loadWord : m -> a -> option (word 32);
+  loadDouble : m -> a -> option (word 64);
+  storeByte : m -> a -> word 8 -> option m;
+  storeHalf : m -> a -> word 16 -> option m;
+  storeWord : m -> a -> word 32 -> option m;
+  storeDouble : m -> a -> word 64 -> option m;
+}.
+
+(* memory addresses are represented using Z because word does not restrict them enough,
+   there are always invalid memory addresses, which are represented by returning None,
+   so we prefer Z, also because that's more "high-level computation" related, where we
+   use Z, rather than "store state" related, where we use word *)
+
+Local Open Scope Z_scope.
+
+Section Memory.
+
+  Variable w: nat. (* bit width of memory words *)
+
+  Definition mem := Z -> option (word w).
+
+  Definition read_mem(x: Z)(m: mem): option (word w) := m x.
+
+  Definition write_mem(x: Z)(v: word w)(m: mem): option mem :=
+    match m x with
+    | Some old_value => Some (fun y => if dec (x = y) then Some v else m y)
+    | None => None
+    end.
+
+  Definition no_mem: mem := fun x => None.
+
+  Definition const_mem(size: Z)(default: word w): mem :=
+    fun x => if dec (x < size) then Some default else None.
+
+  Definition zero_mem(size: Z): mem := const_mem size $0.
+
+  Definition counter_mem(size: Z): mem :=
+    fun x => if dec (x < size) then Some (ZToWord w x) else None.
+
+End Memory.
+
+Arguments read_mem {_} _.
+Arguments write_mem {_} _ _.
+
+Definition read_byte(m: mem 8)(a: Z): option (word 8) := read_mem a m.
+Definition read_half(m: mem 8)(a: Z): option (word 16) :=
+  v0 <- read_byte m a; v1 <- read_byte m (a + 1); Return (combine v0 v1).
+Definition read_word(m: mem 8)(a: Z): option (word 32) :=
+  v0 <- read_half m a; v1 <- read_half m (a + 2); Return (combine v0 v1).
+Definition read_double(m: mem 8)(a: Z): option (word 64) :=
+  v0 <- read_word m a; v1 <- read_word m (a + 4); Return (combine v0 v1).
+
+Definition lobits(sz: nat)(w: word (sz + sz)): word sz := split1 sz sz w.
+Definition hibits(sz: nat)(w: word (sz + sz)): word sz := split2 sz sz w.
+
+Definition write_byte(m: mem 8)(a: Z)(v: word 8): option (mem 8) := write_mem a v m.
+Definition write_half(m: mem 8)(a: Z)(v: word 16): option (mem 8) :=
+  m <- write_byte m a (lobits 8 v); write_byte m (a + 1) (hibits 8 v).
+Definition write_word(m: mem 8)(a: Z)(v: word 32): option (mem 8) :=
+  m <- write_half m a (lobits 16 v); write_half m (a + 2) (hibits 16 v).
+Definition write_double(m: mem 8)(a: Z)(v: word 64): option (mem 8) :=
+  m <- write_word m a (lobits 32 v); write_word m (a + 4) (hibits 32 v).
+
+
+Definition uwordToZ{sz: nat}(w: word sz): Z := Z.of_N (wordToN w).
+
+Definition wrapLoad{aw sz: nat}(f: mem 8 -> Z -> option (word sz))
+  (m: mem 8)(a: word aw): option (word sz) := f m (uwordToZ a).
+
+Definition wrapStore{aw sz: nat}(f: mem 8 -> Z -> word sz -> option (mem 8))
+  (m: mem 8)(a: word aw)(v: word sz): option (mem 8) := f m (uwordToZ a) v.
+
+Instance mem_is_Memory(aw: nat): Memory (mem 8) (word aw) := {|
+  loadByte   := wrapLoad read_byte;
+  loadHalf   := wrapLoad read_half;
+  loadWord   := wrapLoad read_word;
+  loadDouble := wrapLoad read_double;
+  storeByte   := wrapStore write_byte;
+  storeHalf   := wrapStore write_half;
+  storeWord   := wrapStore write_word;
+  storeDouble := wrapStore write_double;
+|}.
+
+
+Section store_retrieve.
+
+  Context {sz: nat}.
+
+  Fixpoint storeWords(l: list (word 32))(a: word sz)(m: mem 8): option (mem 8) :=
+    match l with
+    | nil => Some m
+    | cons w l' =>
+        match storeWord m a w with
+        | Some m' => storeWords l' (a ^+ $4) m'
+        | None => None
+        end
+    end.
+
+  Fixpoint mem_to_word_list(m: mem 8)(start: Z)(count: nat): list (option (word 32)) :=
+    match count with
+    | S c => read_word m start :: mem_to_word_list m (start + 4) c
+    | O => nil
+    end.
+
+  Lemma write_read_byte: forall m m' a v ,
+    write_byte m a v = Some m' ->
+    read_byte m' a = Some v.
+  Proof.
+    intros. unfold write_byte, read_byte, read_mem, write_mem in *.
+    destruct (m a) eqn: E; [|discriminate].
+    inversion H. clear H. subst.
+    match goal with
+    | |- context [@dec ?P ?d] =>
+      let x := constr:(@dec P d) in destruct x; [reflexivity|contradiction]
+    end.
+  Qed.
+
+  Lemma write_read_byte_diff: forall a1 a2 m m' v o,
+    a2 <> a1 ->
+    read_byte m a1 = o ->
+    write_byte m a2 v = Some m' ->
+    read_byte m' a1 = o.
+  Proof.
+    intros. unfold read_byte, write_byte, read_mem, write_mem in *.
+    destruct (m a2) eqn: E; [|discriminate].
+    inversion H1.
+    match goal with
+    | |- context [@dec ?P ?d] =>
+      let x := constr:(@dec P d) in destruct x; [contradiction|assumption]
+    end.
+  Qed.
+
+  Lemma write_read_half: forall m m' a v ,
+    write_half m a v = Some m' ->
+    read_half m' a = Some v.
+  Proof.
+    intros. unfold write_half, read_half in *. simpl in *.
+    match goal with
+    | H: match ?x with _ => _ end = Some _ |- _ => destruct x eqn: E; [|discriminate]
+    end.
+    pose proof H as H'.
+    apply write_read_byte in H'. rewrite H'.
+    pose proof E as E'.
+    apply write_read_byte in E'.
+    assert (a + 1 <> a) as Q by omega.
+    pose proof (write_read_byte_diff a _ m0 m' _ _ Q E' H) as P.
+    rewrite P.
+    f_equal.
+    unfold lobits, hibits.
+    apply combine_split.
+  Qed.
+
+  Lemma write_read_word: forall m m' a v ,
+    write_word m a v = Some m' ->
+    read_word m' a = Some v.
+  Admitted.
+
+  Lemma store_retrieve_word_list: forall l a m m',
+    storeWords l a m = Some m' ->
+    mem_to_word_list m' (uwordToZ a) (length l) = map Some l.
+  Proof.
+    induction l; intros; simpl in *; try reflexivity.
+    destruct (wrapStore write_word m a0 a) eqn: F; [|discriminate].
+    specialize IHl with (1 := H).
+    assert (uwordToZ (a0 ^+ $4) = uwordToZ a0 + 4) as E by admit.
+    rewrite E in IHl.
+    rewrite IHl.
+    f_equal.
+    unfold wrapStore in F.
+  Abort.
+
+End store_retrieve.
